## t1 = λx.x
bound(t1) = { x }
free(t1) = ∅

## t2 = x (λx. y)

bound(t2) = { x }
free(t2)  = { y, x }

bound(λx .y) = bound(y) ∪ { x } = { x }

## substitution

(λx. y)[ x ↦ y ]
** λx is not affected because
   (λy. y) is a different function

(λx. x)[ x ↦ y ]
** the body is not affected because
  (λx. y) is a different function

(λy. y x)[ x ↦ y ]
  ** cannot substitute directly because
     (λy. y y) is a different function

--> (λy′. y′ x)[ x ↦ y ]
    == (λy′. y′ y)

## Diamond Lemma:
If
M →β* M₁
M →β* M₂
then
∃ N such that M₁ →β* N and M₂ →β* N

    M
   / \
  M₁  M₂
   \ /
    N

## Lemma
A lambda term M has at most one normal form.
Suppose M has two normal forms N₁ and N₂

By def: M →β* N₁ and N₁ contains no β redexes
        M →β* N₂ and N₂ contains no β redexes
By (CR or diamond lemma) ∃ N such that
N₁ →β* N and N₂ →β* N
So N₁ =α N₂

## encoding of booleans

IF (λxy.x) M N
== (λb.b) (λxy.x) M N
→β (λxy.x) M N
→β (λy. M) N
→β M

## Church numerals

[1] = λf.λx.f x
[2] = λf.λx. f (f x)

## Successor

SUC [n] →β* [n+1]
SUC = λn. λf. λx. f (n f x)
   or λn. λf. λx. n f (f x)

## Addition

ADD [m] [n] →β* [m+n]
ADD = λm. λn. λf. λx. m f (n f x)

## test for zero

IF0 = λi. i (λ_. FALSE) TRUE

## pairs

FST (PAIR M N)
== (λp. p (λxy. x)) (λv. v M N)
→β (λv. v M N) (λxy. x)
→β (λxy. x) M N
→β→β M

## sums

LEFT = λm. λl. λr. l m
RIGHT = λm. λl. λr. r m
CASE = λv.v

CASE (LEFT M) L R
→β* (λl. λr. l M) L R
→β→β L M


## the fixed point theorem

Y = λ f. (λx.f (x x)) (λx.f (x x))

Y M
→β (λx.M (x x)) (λx.M (x x))
→β M ((λx.M (x x)) (λx.M (x x)))
←β M (Y M)

⇒ Y M is a fixed point of M

## multiplication using fixed point
## Scott encoding
## (x′ + 1) * y = y + (x′ * y)

## without fixed point, using recursion
mul = λ x y. CASE_Nat x |Zero| (λ x′. |add| y (mul x′ y))

## with fixed point
fₘ = λmul. λ x y. CASE_Nat x |Zero| (λ x′. |add| y (mul x′ y))
|mul| = Y fₘ

### unification / unifier

𝓔 = { Bool ≐ Int }
⇒ no unifier exists

𝓔 = { Bool ≐ α }
⇒ S = α ↦ Bool  is most general unifier

𝓔 = { Int → α ≐ β → Bool }
⇒ S = α ↦ Bool, β ↦ Int


𝓔 = { Int → α ≐ Int → β }
⇒ S = α ↦ β           is most general unifier
⇒ S′ = α ↦ T, β ↦ T   is also a unifier for any T
